src/while/fac.v
@@ -3,112 +3,8 @@ From mathcomp Require Import ssreflect eqtype ssrbool seq.
 
 Require Export Arith.
 Require Export ZArith.
-Require Export tactics.
 
-Require Import sem.
-
-Inductive id : Type := Id: nat -> id.
-
-Definition eqid x1 x2 := 
-  match x1 with
-    Id n1 => match x2 with Id n2 => beq_nat n1 n2 end
-  end.
-
-Lemma eqidP : Equality.axiom eqid. 
-Proof.
-  move=>x1 x2.
-  rewrite /eqid; apply: (iffP idP) => [|<-]; last first.
-  - elim x1=>//; apply: Nat.eqb_refl.
-  - elim: x1=> n. elim: x2=> n0.
-    move=> H_eq. apply beq_nat_true in H_eq. 
-    move: H_eq=>->=>//.
-Qed.
-
-Canonical id_eqMixin := EqMixin eqidP.
-Canonical id_eqType := EqType id id_eqMixin. 
-
-Inductive aexp : Type :=
-  ANum: Z -> aexp |
-  AVar: id -> aexp |
-  AAdd: aexp -> aexp -> aexp |
-  ASub: aexp -> aexp -> aexp |
-  AMul: aexp -> aexp -> aexp
-.
-
-Inductive bexp : Type :=
-  BConst: bool -> bexp |
-  BEq: aexp -> aexp -> bexp |
-  BLt: aexp -> aexp -> bexp |
-  BNot: bexp -> bexp |
-  BAnd: bexp -> bexp -> bexp
-.
-
-Definition state := (id -> Z). 
-
-Fixpoint aval (a: aexp) (st: state) : Z :=
-  match a with
-    ANum z => z
-  | AVar x => (st x)
-  | AAdd a1 a2 => (aval a1 st) + (aval a2 st)
-  | ASub a1 a2 => (aval a1 st) - (aval a2 st)
-  | AMul a1 a2 => (aval a1 st) * (aval a2 st) 
-  end.
-
-Fixpoint bval (b: bexp) (st: state) : bool :=
-  match b with
-    BConst v => v
-  | BEq a1 a2 => (Z.eqb (aval a1 st) (aval a2 st))
-  | BLt a1 a2 => (Z.ltb (aval a1 st) (aval a2 st)) 
-  | BNot b0 => if (bval b0 st) then false else true
-  | BAnd b1 b2 =>
-    if (bval b1 st) then
-      (if (bval b2 st) then true else false)
-    else false
-  end. 
-
-Inductive com : Type :=
-  CmSkp: com |
-  CmAssg: id -> aexp -> com |
-  CmIf: bexp -> com -> com -> com |
-  CmWh: bexp -> com -> com |
-  CmSeq: com -> com -> com.
-
-Definition wh_config := (prod com state).
-Definition wh_rconfig := state.
-
-Definition st_upd (s: state) x z :=
-  (fun x' => (if (x == x') then z else (s x'))).
-
-(* the semantic rules *) 
-Inductive wh_rule :
-  seq (prod wh_config wh_rconfig) -> (prod wh_config wh_rconfig) -> Prop :=
-| WHR_SKP s: wh_rule [:: ] ((CmSkp, s), s)
-| WHR_ASSG s x a: wh_rule [:: ] ((CmAssg x a, s), (st_upd s x (aval a s)))
-| WHR_IFTT s s' b c1 c2:
-    bval b s = true -> wh_rule [:: ((c1, s), s')] ((CmIf b c1 c2, s), s')
-| WHR_IFFF s s' b c1 c2: 
-    bval b s = false -> wh_rule [:: ((c2, s), s')] ((CmIf b c1 c2, s), s') 
-| WHR_WHTT s s' s'' b c: 
-    bval b s = true ->
-    wh_rule [:: ((c, s), s''); ((CmWh b c, s''), s')] ((CmWh b c, s), s') 
-| WHR_WHFF s b c:
-    bval b s = false -> wh_rule [:: ] ((CmWh b c, s), s) 
-| WHR_SEQ s s'' s' c1 c2: 
-    wh_rule [:: ((c1, s), s''); ((c2, s''), s')] ((CmSeq c1 c2, s), s')
-.
-
-Instance wh_Sem : Sem wh_config wh_rconfig :=
-  {
-  rule := wh_rule
-  }.
-
-
-Lemma st_upd_eq: forall s x z, (st_upd s x z) x = z.
-Proof. move=> s x z. rewrite /st_upd. elim: eqP=>//. Qed.
-
-Lemma st_upd_neq: forall s x z x', x <> x' -> (st_upd s x z) x' = s x'.
-Proof. move=> s x z x' H_neq. rewrite /st_upd. elim: eqP=>//. Qed. 
-
+From indv Require Import sem tactics lang st_upd. 
 
 (* the factorial program *)
 Definition m: id := Id 0.
@@ -153,62 +49,31 @@ Proof.
   by rewrite <-H; auto with zarith.
 Qed.
 
-Ltac updsimp_h hyp :=
-  repeat (
-      first [
-          rewrite st_upd_eq in hyp |
-          rewrite st_upd_neq in hyp; [| intro H_eq; inversion H_eq ]
-        ]
-    ).
-
-Ltac updsimp :=
-  repeat (
-      first [
-          rewrite st_upd_eq |
-          rewrite st_upd_neq; [| intro H_eq; inversion H_eq ]
-        ]
-    ).
-
 
 (* the correctness proof *)
-  
-Theorem c0_spec_valid: forall param, valid _ (c0_spec param).
+Theorem c0_spec_valid: forall prm, valid _ (c0_spec prm).
 Proof.
   init_verif. 
   inversion H0; subst.
-  -
-    inversion H as [c r' crs H_rule H_all]; subst.
+  - inversion H as [c r' crs H_rule H_all]; subst.
     inversion H_rule; subst.
-    +
-      ith_prem_exe_0 H_all H_i' c0_spec. 
-      ith_prem_exe_0 h H_bd' c0_spec. 
-      ith_prem_exe_1 h H_bd' c0_spec. 
-      clear h0 h1.
-      ith_prem_1 H_all H_all. 
-      inversion H_all.
-      exfalso. apply H2. eexists. eapply WH_SP_c_wh. updsimp.
-      simpl in H4. apply Z.ltb_lt in H4. auto with zarith.
-      inversion H2 as [P [H_spec H_Pr]].
-      inversion H_spec; subst. 
-      updsimp_h H5. inversion H_Pr; subst. updsimp_h H6.
-      unfold c_wh_res. 
+    + prem0_exe H_all. prem0_exe hall. prem1_exe hall. 
+      clear hall0 hall1 hall.
+      prem1_spec H_all. use_spec hspc.
+      { eexists. eapply WH_SP_c_wh. updsimp.
+        simpl in H4. apply Z.ltb_lt in H4. auto with zarith. }
+      updsimp_h H5. unfold c_wh_res. 
       have H_minus_one: (s m - 2)%Z = ((s m - 1) - 1)%Z
         by auto with zarith.
-      rewrite <-facz_unfold; auto with zarith.
-    +
-      simpl in H4. apply Z.ltb_ge in H4.
+      rewrite <-facz_unfold; auto with zarith.      
+    + simpl in H4. apply Z.ltb_ge in H4.
       have H00: (r m = 1)%Z by auto with zarith.
       unfold c_wh_res. rewrite H00. simpl.
       unfold facz; simpl. auto with zarith.
-  -
-    inversion H; subst.
-    inversion H4; subst.
-    ith_prem_exe_0 H5 H5' c0_spec. clear h.
-    ith_prem_1 H5 H5.
-    inversion H5. inversion H2.
-    exfalso. apply H3. eexists. eapply WH_SP_c_wh. updsimp; auto.
-    inversion H2. inversion H3. rename x into P'.
-    inversion H6; subst. inversion H7; subst.
-    updsimp_h H10. 
-    unfold c0_res. rewrite <-facz_unfold; auto.
-Qed. 
+  - inversion H; subst. inversion H4; subst. clear H4.
+    prem0_exe H5. clear hall. prem1_spec H5.
+    use_spec hspc. { eexists. eapply WH_SP_c_wh. updsimp; auto. }
+    unfold c0_res. rewrite H4.
+    updsimp. rewrite facz_unfold; auto.
+Qed.
+
