src/tactics.v
@@ -2,7 +2,8 @@
 Require Import List. 
 From mathcomp Require Import ssreflect seq.
 
-Require Import sem.
+Require Import ZArith.
+From indv Require Import sem.
 
 Ltac inv h := inversion h. 
 
@@ -18,20 +19,44 @@ Ltac ith_prem hyp_alli i p hyp_as :=
   specialize (hyp_alli i p) as hyp_as; simpl in hyp_as;
   rem_hd hyp_as; clear hyp_as; intro hyp_as.
 
-Ltac ith_prem_exe hyp_alli i p hyp_as spec :=
-  let h := fresh "h" in (
-    ith_prem hyp_alli i p hyp_as; 
-    inversion hyp_as as [H_nex | H_ex]; clear hyp_as;
-    [
-      inversion H_nex as [H_ne H_inf']; clear H_nex H_ne;
-      inversion H_inf' as [c r' crs H_rule' h]; subst; clear H_inf';
-      inversion H_rule'; subst; clear H_rule' |      
-      inversion H_ex; 
-      match goal with | [ H: spec _ _ _ /\ _ |- _ ] => inversion H end;
-      match goal with | [ H: spec _ _ _ |- _ ] => inversion H end
-  ]).
+Ltac ith_prem_spec hyp_alli i p :=
+  let hypas := fresh "hypas" with
+    hspc := fresh "hspc" with
+    hexe := fresh "hexe"
+                 in (
+                     specialize (hyp_alli i p) as hypas; simpl in hypas;
+                     rem_hd hypas; clear hypas; intro hypas;
+                     inversion hypas as [hspc hexe]; clear hypas; clear hexe
+                   ).
 
-Ltac ith_prem_0 hyp_alli hyp_as :=
+Ltac ith_prem_exe hyp_alli i p :=
+  let hypas := fresh "hypas" with
+    hallP := fresh "hallP" with
+    hnexP := fresh "hnexP" with
+    hp := fresh "hp" with
+    pp := fresh "pp" with
+    hpp := fresh "hpp" with 
+    hinf := fresh "hinf" with
+    cc := fresh "cc" with 
+    rr := fresh "rr" with
+    crs := fresh "crs" with
+    hrule := fresh "hrule" with
+    hall := fresh "hall"
+                 in (
+                     ith_prem hyp_alli i p hypas; 
+                     inversion hypas as [hallP hnexP];
+                     clear hypas hallP;
+                     (match type of hnexP with
+                      | _ -> ?P => (
+                          have: P by
+                            (apply hnexP; intro hp; inversion hp as [pp hpp];
+                             inversion hpp))
+                      end;
+                      clear hnexP; intro hinf;
+                      inversion hinf as [cc rr crs hrule hall]; subst; clear hinf;
+                      inversion hrule; subst; clear hrule)). 
+
+Ltac prem0 hyp_alli hyp_as :=
   match type of hyp_alli with
     (forall _ _, nth_error ?lst _ = _ -> _) => (
       match lst with
@@ -41,7 +66,17 @@ Ltac ith_prem_0 hyp_alli hyp_as :=
     )
   end.
 
-Ltac ith_prem_1 hyp_alli hyp_as :=
+Ltac prem0_spec hyp_alli :=
+  match type of hyp_alli with
+    (forall _ _, nth_error ?lst _ = _ -> _) => (
+      match lst with
+        nil => idtac
+      | ?p :: _ => ith_prem_spec hyp_alli 0 p 
+      end
+    )
+  end.
+
+Ltac prem1 hyp_alli hyp_as :=
   match type of hyp_alli with
   | (forall _ _, nth_error ?lst _ = _ -> _) => (
       match lst with
@@ -54,7 +89,20 @@ Ltac ith_prem_1 hyp_alli hyp_as :=
       end)
   end.
 
-Ltac ith_prem_2 hyp_alli hyp_as :=
+Ltac prem1_spec hyp_alli :=
+  match type of hyp_alli with
+  | (forall _ _, nth_error ?lst _ = _ -> _) => (
+      match lst with
+        nil => idtac
+      | ?p :: ?lst' => (
+          match lst' with
+            nil => idtac
+          | ?p' :: ?lst'' => ith_prem_spec hyp_alli 1 p' 
+          end)
+      end)
+  end.
+
+Ltac prem2 hyp_alli hyp_as :=
   match type of hyp_alli with
   | (forall _ _, nth_error ?lst _ = _ -> _) => (
       match lst with
@@ -69,19 +117,36 @@ Ltac ith_prem_2 hyp_alli hyp_as :=
               end)
           end)
       end)
+  end.
+
+Ltac prem2_spec hyp_alli :=
+  match type of hyp_alli with
+  | (forall _ _, nth_error ?lst _ = _ -> _) => (
+      match lst with
+        nil => idtac
+      | ?p :: ?lst' => (
+          match lst' with
+            nil => idtac
+          | ?p' :: ?lst'' => (
+              match lst'' with
+                nil => idtac
+              | ?p'' :: ?lst''' => ith_prem_spec hyp_alli 2 p'' 
+              end)
+          end)
+      end)
   end. 
   
-Ltac ith_prem_exe_0 hyp_alli hyp_as spec :=
+Ltac prem0_exe hyp_alli :=
   let h := fresh "h" in (
     match type of hyp_alli with
     | (forall _ _, nth_error ?lst _ = _ -> _) => (
         match lst with
           nil => idtac 
-        | ?p :: _ => ith_prem_exe hyp_alli 0 p hyp_as spec
+        | ?p :: _ => ith_prem_exe hyp_alli 0 p 
         end)
     end).
 
-Ltac ith_prem_exe_1 hyp_alli hyp_as spec :=
+Ltac prem1_exe hyp_alli :=
   let h := fresh "h" in (
     match type of hyp_alli with
     | (forall _ _, nth_error ?lst _ = _ -> _) => (
@@ -90,12 +155,12 @@ Ltac ith_prem_exe_1 hyp_alli hyp_as spec :=
         | ?p :: ?lst' => (
             match lst' with
               nil => idtac
-            | ?p' :: ?lst'' => ith_prem_exe hyp_alli 1 p' hyp_as spec
+            | ?p' :: ?lst'' => ith_prem_exe hyp_alli 1 p' 
             end)
         end)
     end).
 
-Ltac ith_prem_exe_2 hyp_alli hyp_as spec :=
+Ltac prem2_exe hyp_alli :=
   let h := fresh "h" in (
     match type of hyp_alli with
     | (forall _ _, nth_error ?lst _ = _ -> _) => (
@@ -108,9 +173,55 @@ Ltac ith_prem_exe_2 hyp_alli hyp_as spec :=
                 match lst'' with
                   nil => idtac
                 | ?p'' :: ?lst''' =>
-                  ith_prem_exe hyp_alli 2 p'' hyp_as spec
+                  ith_prem_exe hyp_alli 2 p'' 
                 end)
             end)
         end)
     end).
 
+Ltac assert_in_spc hyp_spc := 
+  match type of hyp_spc with
+    forall P, ?S ?a ?b P -> P _ =>
+    have: exists P, S a b P
+  end.
+
+(* hex is the proposition saying that pp is a set of result configs 
+   given by the specification *)
+Ltac use_spec hyp_spc :=
+  let pp := fresh "pp" with hex := fresh "hex"
+              in (
+                  assert_in_spc hyp_spc;
+                  [ |
+                    elim=> [pp hex];
+                           specialize (hyp_spc pp hex);
+                           inversion hex; subst; clear hex;
+                           inversion hyp_spc; subst; clear hyp_spc]).
+
+
+Ltac rem_prem hyp :=
+  match type of hyp with
+  | _ -> ?P => have: P; [apply hyp=>// | ]=>{hyp}=>hyp
+  end.
+
+(* solve goal with contradicting hypothesis of the forms 
+   (a < b)%Z and (b <= a)%Z *) 
+Ltac comp_contra hyp1 hyp2 :=
+  let contra := fresh "contra" in (
+    match type of hyp1 with
+      (?x < ?y)%Z => (
+        specialize (Z.lt_le_trans _ _ _ hyp1 hyp2)
+        => contra; apply Z.lt_irrefl in contra; inv contra)
+    | (?x <= ?y)%Z => (
+        specialize (Z.le_lt_trans _ _ _ hyp1 hyp2)
+        => contra; apply Z.lt_irrefl in contra; inv contra)
+    end
+  ).
+
+Ltac some_eq hyp1 hyp2 :=
+  first [
+      rewrite hyp1 in hyp2; inv hyp2; auto |
+      rewrite <- hyp1 in hyp2; inv hyp2; auto |
+      rewrite hyp2 in hyp1; inv hyp1; auto |
+      rewrite <- hyp2 in hyp2; inv hyp1; auto
+    ].
+            
